WIP matches_spec

Clap/Lang/F/F.lean
@@ -1,18 +1,113 @@
 import Clap.eDSLState.eDSL
+import Clap.eDSLState.IsValid
 
 import Clap.Lang.Wheels
 
-namespace Clap.Edsl.Lang
+namespace Clap.Lang
 
-abbrev F p := FixedExp p
+abbrev F := ExprRef -- TODO Expr or ExprRef?
+abbrev FB := F
 
 namespace F
 
 variable {p : ℕ}
 
-def isValid (x : F p) (varStore : VarStore p) : Prop :=
-  (x.eval varStore).isSome
+instance : IsValid p F where
+  isValid Γ σ x := [Γ,σ|x].isSome = true
+
+open HashConsM in
+def eq {p : ℕ} [p.AtLeastTwo] (a b : F) : ClapM p FB := do
+  isZero (←mkSub (p := p) a b)
+
+open HashConsM in
+def oneHotRaw [p.AtLeastTwo] (len : ℕ) (idx : F) : ClapM p (Vector FB len) :=
+  (Vector.range len).mapM (fun (i:ℕ) ↦ do
+    let idx_val ← mkConstant (p := p) i
+    F.eq idx idx_val
+  )
+
+def matches_spec
+  [p.AtLeastTwo]
+  (varStore : VarStore p)
+  (numAlloc : ℕ)
+  (σ : HashConsSt p)
+  {α β}
+  (toIdeal : VarStore p → HashConsSt p → α → Option β)
+  (cmd : ClapM p α)
+  (spec : β)
+: Prop :=
+  let result := cmd.getResult numAlloc σ
+  let varStorePost := [varStore, cmd.getHashConsState numAlloc σ, numAlloc|cmd.getCircuit numAlloc σ]ₑ.varStore
+  let σPost := cmd.getHashConsState numAlloc σ
+  toIdeal varStorePost σPost result = .some spec ∧
+  cmd.wellFormed numAlloc varStore σ
+
+namespace eq
+
+opaque spec {p} (a b : ZMod p) : Bool :=
+  a == b
+
+opaque Convert.toIdeal (varStore : VarStore p) (σ : HashConsSt p) (result : FB) : Option Bool
+
+lemma matches_spec
+  [p.AtLeastTwo]
+  {varStore : VarStore p}
+  {numAlloc : ℕ}
+  {σ : HashConsSt p}
+  (a b : F)
+  (a_val b_val : ZMod p)
+  (h_a_wf : [varStore|Expr.mk a σ].isSome = true)
+  (h_a_val : [varStore,σ|a].get h_a_wf = a_val)
+  (h_b_wf : [varStore|Expr.mk b σ].isSome = true)
+  (h_b_val : [varStore,σ|b].get h_b_wf = b_val)
+:
+  F.matches_spec
+    varStore
+    numAlloc
+    σ
+    Convert.toIdeal
+    (eq a b)
+    (spec a_val b_val)
+:= by
+  sorry
+
+end eq
+
+namespace oneHotRaw
+
+opaque spec (len : ℕ) (idx : ℕ) : Vector Bool len :=
+  (Vector.range len).map (fun (i:ℕ) ↦ idx == i)
+
+opaque Convert.toIdeal {len : ℕ} (varStore : VarStore p) (σ : HashConsSt p) (result : Vector FB len) : Option (Vector Bool len)
+
+
+--TODO prove using eq.matches_spec
+--this may require adding to F.matches_spec, or defining properties about Convert.toIdeal
+--in either case, the goal is to reach a fixed point where the same properties are known about the two Convert.toIdeal functions,
+--and the same F.matches_spec is being used for eq and proven for oneHotRaw
+lemma matches_spec
+  [p.AtLeastTwo]
+  {len : ℕ}
+  {idx : F}
+  {varStore : VarStore p}
+  {numAlloc : ℕ}
+  {σ : HashConsSt p}
+  {idx_val : ℕ}
+  (h_idx_wf : [varStore|Expr.mk idx σ].isSome = true)
+  (h_idx_val : ([varStore,σ|idx].get h_idx_wf).val = idx_val)
+:
+  F.matches_spec
+    varStore
+    numAlloc
+    σ
+    Convert.toIdeal
+    (oneHotRaw len idx)
+    (spec len idx_val)
+:= by
+  done
+
+end oneHotRaw
 
 end F
 
-end Clap.Edsl.Lang
+end Clap.Lang
