Clap/Lang/FArray/OneHotRaw.lean
@@ -4,236 +4,240 @@ namespace Clap.Edsl.Lang.FArray
 
 variable {p : ℕ}
 
-def oneHotRaw [p.AtLeastTwo] (len : ℕ) (idx : F p) : Edsl.CircuitM p (Vector (FB p) len) :=
+def oneHotRaw [p.AtLeastTwo] (len : ℕ) (idx : F p) : ClapM p (Vector (FB p) len) :=
   (Vector.range len).mapM (fun (i:ℕ) ↦ F.eq idx i)
 
 namespace oneHotRaw
 
-def runAndEval
-  {p : ℕ} {ResultT : Type} (cmd : CircuitM p ResultT) (numAlloc : ℕ) (varStore : Std.ExtTreeMap ℕ (ZMod p))
+lemma spec
 :
-  ResultT × CircuitResult p
-:=
-  let ⟨⟨result, circuit⟩, _numAlloc⟩ := (cmd.run numAlloc)
-  ⟨result, Edsl.Circuit.eval circuit varStore numAlloc⟩
+  oneHotRaw len
+
+-- def runAndEval
+--   {p : ℕ} {ResultT : Type} (cmd : CircuitM p ResultT) (numAlloc : ℕ) (varStore : Std.ExtTreeMap ℕ (ZMod p))
+-- :
+--   ResultT × CircuitResult p
+-- :=
+--   let ⟨⟨result, circuit⟩, _numAlloc⟩ := (cmd.run numAlloc)
+--   ⟨result, Edsl.Circuit.eval circuit varStore numAlloc⟩
 
 
--- def matchesUnaryBitVecFunctionWithSideEffects
---   {length: ℕ}
---   (p : ℕ)
---   [p.AtLeastTwo]
---   (spec_function : (ZMod p) → Vector Bool length)
---   (function : (F p) → Edsl.CircuitM p (Vector (FB p) length))
---   (allocates : ℕ)
--- : Prop :=
---   ∀ (a : F p) varStorePre numAllocPre,
---   a.isValid (varStorePre.get?) →
---   let a_eval := (a.eval varStorePre.get?).getD 0
---   let ⟨result, numAllocPost, varStorePost, constraints⟩ := runAndEval (function a) numAllocPre varStorePre
---   result.map (FB.toBool · varStorePost.get?) = spec_function a_eval ∧
---   constraints = True ∧
---   numAllocPost = numAllocPre + allocates ∧
---   ∀ i < numAllocPre, varStorePost.get? i = varStorePre.get? i ∧
---   ∀ (i: Fin length),
---     varStorePost.get? (numAllocPost - i) =
---     .some (((spec_function a_eval).get ⟨length - 1 - i, by {
---       omega
---     }⟩).toNat)
+-- -- def matchesUnaryBitVecFunctionWithSideEffects
+-- --   {length: ℕ}
+-- --   (p : ℕ)
+-- --   [p.AtLeastTwo]
+-- --   (spec_function : (ZMod p) → Vector Bool length)
+-- --   (function : (F p) → Edsl.CircuitM p (Vector (FB p) length))
+-- --   (allocates : ℕ)
+-- -- : Prop :=
+-- --   ∀ (a : F p) varStorePre numAllocPre,
+-- --   a.isValid (varStorePre.get?) →
+-- --   let a_eval := (a.eval varStorePre.get?).getD 0
+-- --   let ⟨result, numAllocPost, varStorePost, constraints⟩ := runAndEval (function a) numAllocPre varStorePre
+-- --   result.map (FB.toBool · varStorePost.get?) = spec_function a_eval ∧
+-- --   constraints = True ∧
+-- --   numAllocPost = numAllocPre + allocates ∧
+-- --   ∀ i < numAllocPre, varStorePost.get? i = varStorePre.get? i ∧
+-- --   ∀ (i: Fin length),
+-- --     varStorePost.get? (numAllocPost - i) =
+-- --     .some (((spec_function a_eval).get ⟨length - 1 - i, by {
+-- --       omega
+-- --     }⟩).toNat)
 
-def specFunction (n : ℕ) : Fin n → Vector Bool n := fun i ↦
-  Vector.ofFn λ (idx : Fin n) => idx.val == i
+-- def specFunction (n : ℕ) : Fin n → Vector Bool n := fun i ↦
+--   Vector.ofFn λ (idx : Fin n) => idx.val == i
 
-def isValidRange (varStore : VarStore p) (x : F p) (lt : ℕ) : Prop :=
-  (x.eval varStore).any (λ val => val.val < lt)
+-- def isValidRange (varStore : VarStore p) (x : F p) (lt : ℕ) : Prop :=
+--   (x.eval varStore).any (λ val => val.val < lt)
 
-lemma eval_of_isValidRange
-  {varStore : VarStore p}
-  {x : F p}
-  {lt : ℕ}
-  (h: isValidRange varStore x lt)
-:
-  ∃ val, x.eval varStore = .some val ∧ val.val < lt
-:= by
-  unfold isValidRange at h
-  grind [Option.any_eq_true]
+-- lemma eval_of_isValidRange
+--   {varStore : VarStore p}
+--   {x : F p}
+--   {lt : ℕ}
+--   (h: isValidRange varStore x lt)
+-- :
+--   ∃ val, x.eval varStore = .some val ∧ val.val < lt
+-- := by
+--   unfold isValidRange at h
+--   grind [Option.any_eq_true]
 
--- TODO there must surely be a better name for this
--- DONE Yes, it's this name.
-lemma val_get_eval_mod_lt
-  {varStore : VarStore p}
-  {k : ℕ}
-  {x : F p}
-  {h : (FixedExp.eval varStore x).isSome = true}
-  [Fact (k ≤ p)]
-  (h_isValid : isValidRange varStore x k)
-:
-  ((x.eval varStore).get h).val % p < k
-:= by
-  apply Nat.mod_lt_of_lt
-  grind [eval_of_isValidRange]
+-- -- TODO there must surely be a better name for this
+-- -- DONE Yes, it's this name.
+-- lemma val_get_eval_mod_lt
+--   {varStore : VarStore p}
+--   {k : ℕ}
+--   {x : F p}
+--   {h : (FixedExp.eval varStore x).isSome = true}
+--   [Fact (k ≤ p)]
+--   (h_isValid : isValidRange varStore x k)
+-- :
+--   ((x.eval varStore).get h).val % p < k
+-- := by
+--   apply Nat.mod_lt_of_lt
+--   grind [eval_of_isValidRange]
 
-attribute [local grind _=_] Array.toList_mapM Vector.toArray_mapM
-attribute [local grind =] Vector.map_id_fun Vector.map_id ZMod.val_natCast
-attribute [local grind .] Vector.mem_toArray_iff
+-- attribute [local grind _=_] Array.toList_mapM Vector.toArray_mapM
+-- attribute [local grind =] Vector.map_id_fun Vector.map_id ZMod.val_natCast
+-- attribute [local grind .] Vector.mem_toArray_iff
 
-instance {k p} [inst_lt : Fact (k ≤ p)] : FB.Convert p (F p) (Fin k) where
-  isValid varStore x :=
-    isValidRange varStore x k
-  size :=
-    1
-  toLinear varStore x :=
-    #v[x.eval varStore |>.getD 42]
-  toIdeal varStore x :=
-    (x.eval varStore).bind (λ x => if h: x.val < k then .some ⟨x.val, h⟩ else .none)
-  toRepresents x :=
-    x.val
-  isValid_iff_isSome_toIdeal varStore x h_isValid := by
-    grind [eval_of_isValidRange]
-  toIdealtoRepresents varStore x := by
-    simp [Nat.mod_eq_of_lt (lt_of_lt_of_le x.2 inst_lt.out)]
-  toRepresentstoIdeal varStore x h_isValidRange:= by
-    obtain ⟨x, ⟨h_some, h_range⟩⟩ := eval_of_isValidRange h_isValidRange
-    have : x.val % p = x.val := Nat.mod_eq_of_lt (Nat.lt_of_lt_of_le h_range inst_lt.out)
-    grind
+-- instance {k p} [inst_lt : Fact (k ≤ p)] : FB.Convert p (F p) (Fin k) where
+--   isValid varStore x :=
+--     isValidRange varStore x k
+--   size :=
+--     1
+--   toLinear varStore x :=
+--     #v[x.eval varStore |>.getD 42]
+--   toIdeal varStore x :=
+--     (x.eval varStore).bind (λ x => if h: x.val < k then .some ⟨x.val, h⟩ else .none)
+--   toRepresents x :=
+--     x.val
+--   isValid_iff_isSome_toIdeal varStore x h_isValid := by
+--     grind [eval_of_isValidRange]
+--   toIdealtoRepresents varStore x := by
+--     simp [Nat.mod_eq_of_lt (lt_of_lt_of_le x.2 inst_lt.out)]
+--   toRepresentstoIdeal varStore x h_isValidRange:= by
+--     obtain ⟨x, ⟨h_some, h_range⟩⟩ := eval_of_isValidRange h_isValidRange
+--     have : x.val % p = x.val := Nat.mod_eq_of_lt (Nat.lt_of_lt_of_le h_range inst_lt.out)
+--     grind
 
-@[grind _=_]
-lemma _root_.Vector.isSome_mapM_eq_all_isSome
-  {elemT resultT}
-  {length}
-  {f : elemT → Option resultT}
-  {xs : Vector elemT length}
-:
-  (Vector.mapM f xs).isSome =
-  (xs.map f).all Option.isSome
-:= by
-  have :
-    (Vector.mapM f xs).isSome =
-    (Vector.toArray <$> (Vector.mapM f xs)).isSome
-  := by grind
-  rewrite [this]; clear this
-  simp
-  rewrite [Array.mapM_eq_mapM_toList]
-  have :
-    xs.toArray.toList = xs.toList
-  := rfl
-  rewrite [this]; clear this
-  have :
-    (xs.all λ a => (f a).isSome) =
-    xs.toList.all fun a => (f a).isSome
-  := by
-    rw [←Vector.all_toList]
-  rewrite [this]; clear this
-  induction xs.toList with
-  | nil => simp
-  | cons head tail h_tail =>
-    simp
-    cases (f head) with
-    | none => simp
-    | some head =>
-      rewrite [←h_tail]
-      simp
-      cases (List.mapM f tail) with
-      | none => grind
-      | some rest => grind
+-- @[grind _=_]
+-- lemma _root_.Vector.isSome_mapM_eq_all_isSome
+--   {elemT resultT}
+--   {length}
+--   {f : elemT → Option resultT}
+--   {xs : Vector elemT length}
+-- :
+--   (Vector.mapM f xs).isSome =
+--   (xs.map f).all Option.isSome
+-- := by
+--   have :
+--     (Vector.mapM f xs).isSome =
+--     (Vector.toArray <$> (Vector.mapM f xs)).isSome
+--   := by grind
+--   rewrite [this]; clear this
+--   simp
+--   rewrite [Array.mapM_eq_mapM_toList]
+--   have :
+--     xs.toArray.toList = xs.toList
+--   := rfl
+--   rewrite [this]; clear this
+--   have :
+--     (xs.all λ a => (f a).isSome) =
+--     xs.toList.all fun a => (f a).isSome
+--   := by
+--     rw [←Vector.all_toList]
+--   rewrite [this]; clear this
+--   induction xs.toList with
+--   | nil => simp
+--   | cons head tail h_tail =>
+--     simp
+--     cases (f head) with
+--     | none => simp
+--     | some head =>
+--       rewrite [←h_tail]
+--       simp
+--       cases (List.mapM f tail) with
+--       | none => grind
+--       | some rest => grind
 
-@[grind =_]
-lemma toIdeal_eq_pure_get_of_isValid
-  {representsT idealT}
-  {varStore : VarStore p}
-  {x : representsT}
-  [FB.Convert p representsT idealT]
-  (h : FB.IsValid.isValid varStore x)
-:
-  FB.Convert.toIdeal varStore x =
-  pure ((FB.Convert.toIdeal varStore x).get (FB.Convert.isValid_iff_isSome_toIdeal varStore x h))
-:= by
-  simp
+-- @[grind =_]
+-- lemma toIdeal_eq_pure_get_of_isValid
+--   {representsT idealT}
+--   {varStore : VarStore p}
+--   {x : representsT}
+--   [FB.Convert p representsT idealT]
+--   (h : FB.IsValid.isValid varStore x)
+-- :
+--   FB.Convert.toIdeal varStore x =
+--   pure ((FB.Convert.toIdeal varStore x).get (FB.Convert.isValid_iff_isSome_toIdeal varStore x h))
+-- := by
+--   simp
 
-@[grind =]
-lemma _root_.List.mapM_toRepresentstoIdeal
-  {representsT idealT}
-  {varStore : VarStore p}
-  {xs : List representsT}
-  [base : FB.Convert p representsT idealT]
-  {h}
-:
-  List.mapM (base.toIdeal varStore ∘ base.toRepresents)
-    ((List.mapM (FB.Convert.toIdeal varStore) xs).get h) =
-  List.mapM (FB.Convert.toIdeal varStore) xs
-:= by
-  induction xs with
-  | nil => simp
-  | cons head tail h_tail =>
-    simp [h_tail, base.toIdealtoRepresents]
+-- @[grind =]
+-- lemma _root_.List.mapM_toRepresentstoIdeal
+--   {representsT idealT}
+--   {varStore : VarStore p}
+--   {xs : List representsT}
+--   [base : FB.Convert p representsT idealT]
+--   {h}
+-- :
+--   List.mapM (base.toIdeal varStore ∘ base.toRepresents)
+--     ((List.mapM (FB.Convert.toIdeal varStore) xs).get h) =
+--   List.mapM (FB.Convert.toIdeal varStore) xs
+-- := by
+--   induction xs with
+--   | nil => simp
+--   | cons head tail h_tail =>
+--     simp [h_tail, base.toIdealtoRepresents]
 
-@[grind .]
-lemma _root_.List.isSome_mapM_of_isSome
-  {T T'}
-  {list : List T}
-  {f : T → Option T'}
-  (h : ∀ x ∈ list, (f x).isSome)
-:
-  (List.mapM f list).isSome
-:= by
-  induction list with
-  | nil => simp
-  | cons head tail h_tail =>
-    have h_head := h head (by simp)
-    obtain ⟨head, h_head⟩ := Option.isSome_iff_exists.mp h_head
-    simp [h_head]
-    simp_all -- forgive me
-    obtain ⟨tail, h_tail⟩ := Option.isSome_iff_exists.mp h_tail
-    simp [h_tail]
+-- @[grind .]
+-- lemma _root_.List.isSome_mapM_of_isSome
+--   {T T'}
+--   {list : List T}
+--   {f : T → Option T'}
+--   (h : ∀ x ∈ list, (f x).isSome)
+-- :
+--   (List.mapM f list).isSome
+-- := by
+--   induction list with
+--   | nil => simp
+--   | cons head tail h_tail =>
+--     have h_head := h head (by simp)
+--     obtain ⟨head, h_head⟩ := Option.isSome_iff_exists.mp h_head
+--     simp [h_head]
+--     simp_all -- forgive me
+--     obtain ⟨tail, h_tail⟩ := Option.isSome_iff_exists.mp h_tail
+--     simp [h_tail]
 
-instance
-  {representsT idealT length}
-  [base: FB.Convert p representsT idealT]
-: FB.Convert p (Vector representsT length) (Vector idealT length) where
-  isValid varStore xs :=
-    ∀ x ∈ xs, base.isValid varStore x
-  size := length * base.size
-  toLinear varStore xs :=
-    xs.flatMap (base.toLinear varStore)
-  toIdeal varStore xs :=
-    let ideals := xs.map (base.toIdeal varStore)
-    ideals.mapM id
-  toRepresents xs :=
-    xs.map base.toRepresents
-  isValid_iff_isSome_toIdeal varStore x h_isValid := by
-    grind
-  toIdealtoRepresents varStore xs := by
-    simp only [Function.comp_def, Vector.mapM_map]
-    have := Vector.mapM_pure (m := Option) (xs := xs) (id : idealT → idealT)
-    grind
-  toRepresentstoIdeal varStore xs h := by
-    simp
-    rewrite [←Vector.map_toArray_inj, ←Array.map_toList_inj]
-    simp
-    have (h : (Vector.mapM (FB.Convert.toIdeal varStore) xs).isSome) (h') :
-      ((Vector.mapM (base.toIdeal varStore) xs).get h).toArray.toList =
-      (Array.toList <$> Vector.toArray <$> (Vector.mapM (base.toIdeal varStore) xs)).get h'
-    := by
-      grind
-    grind
+-- instance
+--   {representsT idealT length}
+--   [base: FB.Convert p representsT idealT]
+-- : FB.Convert p (Vector representsT length) (Vector idealT length) where
+--   isValid varStore xs :=
+--     ∀ x ∈ xs, base.isValid varStore x
+--   size := length * base.size
+--   toLinear varStore xs :=
+--     xs.flatMap (base.toLinear varStore)
+--   toIdeal varStore xs :=
+--     let ideals := xs.map (base.toIdeal varStore)
+--     ideals.mapM id
+--   toRepresents xs :=
+--     xs.map base.toRepresents
+--   isValid_iff_isSome_toIdeal varStore x h_isValid := by
+--     grind
+--   toIdealtoRepresents varStore xs := by
+--     simp only [Function.comp_def, Vector.mapM_map]
+--     have := Vector.mapM_pure (m := Option) (xs := xs) (id : idealT → idealT)
+--     grind
+--   toRepresentstoIdeal varStore xs h := by
+--     simp
+--     rewrite [←Vector.map_toArray_inj, ←Array.map_toList_inj]
+--     simp
+--     have (h : (Vector.mapM (FB.Convert.toIdeal varStore) xs).isSome) (h') :
+--       ((Vector.mapM (base.toIdeal varStore) xs).get h).toArray.toList =
+--       (Array.toList <$> Vector.toArray <$> (Vector.mapM (base.toIdeal varStore) xs)).get h'
+--     := by
+--       grind
+--     grind
 
-def spec (p : ℕ) (length : ℕ) [p.AtLeastTwo] [Fact (length ≤ p)] : Prop :=
-  Clap.Edsl.Lang.FB.matchesUnaryMonadFunction
-  p
-  (specFunction length)
-  (oneHotRaw length)
-  length
+-- def spec (p : ℕ) (length : ℕ) [p.AtLeastTwo] [Fact (length ≤ p)] : Prop :=
+--   Clap.Edsl.Lang.FB.matchesUnaryMonadFunction
+--   p
+--   (specFunction length)
+--   (oneHotRaw length)
+--   length
 
-lemma equiv (p : ℕ) (length : ℕ) [p.AtLeastTwo] :
-  spec p length
-:= by
-  unfold spec
-  intro a varStorePre numAllocPre h_a_isValid
-  obtain ⟨a_eval, h_a_eval⟩ := Option.isSome_iff_exists.mp h_a_isValid
-  aesop (add simp [
-    Clap.monads,
-    oneHotRaw,
-    F.eq.equiv
-  ]) (add safe (by grind))
+-- lemma equiv (p : ℕ) (length : ℕ) [p.AtLeastTwo] :
+--   spec p length
+-- := by
+--   unfold spec
+--   intro a varStorePre numAllocPre h_a_isValid
+--   obtain ⟨a_eval, h_a_eval⟩ := Option.isSome_iff_exists.mp h_a_isValid
+--   aesop (add simp [
+--     Clap.monads,
+--     oneHotRaw,
+--     F.eq.equiv
+--   ]) (add safe (by grind))
 
 end oneHotRaw
 
