Clap/Lang/FB/FB.lean
@@ -1,306 +1,322 @@
 import Clap.Lang.F.F
-import Clap.eDSLState.Spec
+import Clap.eDSLState.Convert
 
-namespace Clap.Edsl.Lang
+namespace Clap.Lang
 
 abbrev FB p := F p
 
 namespace FB
 
-def true (p : ℕ) [p.AtLeastTwo] : FB p := .c 1
-def false (p : ℕ) [p.AtLeastTwo] : FB p := .c 0
+instance (p : ℕ) : IsValid p (FB p) where
+  isValid Γ x := [Γ|x] = .some 0 ∨
+                 [Γ|x] = .some 1
 
-@[grind =]
-lemma eval_true {p : ℕ} {varStore : VarStore p} [p.AtLeastTwo]:
-  [varStore|true p] = .some 1
-:= by
-  simp [FB.true]
+-- REVIEW, seems contrived
+def true (p : ℕ) [p.AtLeastTwo] : HashConsM p (FB p) := do
+  let x ← HashConsM.mkConstant 1
+  return ⟨x, ←get⟩
 
-@[grind =]
-lemma eval_false {p : ℕ} {varStore : VarStore p} [p.AtLeastTwo]:
-  [varStore|false p] = .some 0
-:= by
-  simp [FB.false]
+def false (p : ℕ) [p.AtLeastTwo] : HashConsM p (FB p) := do
+  let x ← HashConsM.mkConstant 1
+  return ⟨x, ←get⟩
 
-@[simp, grind =]
-lemma eval_true_isSome {p : ℕ} {varStore : VarStore p} [p.AtLeastTwo]:
-  [varStore|true p].isSome = Bool.true
-:= by
-  grind
+-- instance (p : ℕ) [p.AtLeastTwo] : Convert p (FB p) Bool where
+--   toIdeal Γ x := [Γ|x].bind (λ x => if x == 1 then Bool.true else if x == 0 then Bool.false else .none)
+--   toRepresents b := if b then (FB.true p).run' (.empty p) else (FB.true p).run' (.empty p)
+--   isValid_iff_isSome_toIdeal := sorry
+--   toIdeal_toRepresents := sorry
 
-@[simp, grind =]
-lemma eval_false_isSome {p : ℕ} {varStore : VarStore p} [p.AtLeastTwo]:
-  [varStore|false p].isSome = Bool.true
-:= by
-  grind
-
-variable {p : ℕ} [p.AtLeastTwo]
-
-def isValid (x : FB p) (varStore : VarStore p) : Prop :=
-  x.eval varStore = .some 0 ∨
-  x.eval varStore = .some 1
-
--- TODO there must be a better way of putting this
--- Well, this is just `isValid_iff` with an extra step.
--- I think this is good, and it `simp`s down to `true | false` via `eval_<t|f>`.
-@[grind .]
-lemma isValid_iff_eval_eq_eval_false_or_eval_true
-  {x : FB p} {varStore : VarStore p}
-:
-  x.isValid varStore ↔ (
-    [varStore|x =Γ false p] ∨
-    [varStore|x =Γ true p]
-  )
-:= by
-  simp [isValid, eval_true, eval_false]
-
-def isAlwaysValid (x : FB p) : Prop :=
-  ∀ varStore, x.isValid varStore
-
-def toBool (x : FB p) (varStore : VarStore p) : Option Bool :=
-  [varStore|x].bind (λ x => if x == 1 then Bool.true else if x == 0 then Bool.false else .none)
-
-@[grind .]
-lemma toBool_isSome_eq_true_of_isValid
-  {x : FB p} {varStore : VarStore p}
-  (h_isValid : x.isValid varStore)
-:
-  (x.toBool varStore).isSome = Bool.true
-:= by
-  grind [toBool]
-
-omit [p.AtLeastTwo] in
-@[grind .]
-lemma toBool_isSome_eq_false_of_isValid
-  {x : FB p} {varStore : VarStore p}
-  (h_isValid : ¬x.isValid varStore)
-:
-  (x.toBool varStore).isSome = Bool.false
-:= by
-  simp [isValid] at h_isValid
-  unfold toBool
-  set y := [varStore|x]
-  obtain _ | ⟨y⟩ := y <;> grind
-
-def ofBool (p : ℕ) [p.AtLeastTwo] (x : Bool) : FB p :=
-  if x then FB.true p else FB.false p
-
-@[simp, grind =]
-lemma eval_ofBool {p : ℕ} {varStore : VarStore p} [p.AtLeastTwo] {b : Bool} :
-  [varStore|ofBool p b] = if b then [varStore|true p] else [varStore|false p]
-:= by
-  grind [FB.ofBool]
-
-@[simp, grind =]
-lemma toBool_ofBool
-  {p : ℕ}
-  {varStore : VarStore p}
-  (b: Bool)
-  [p.AtLeastTwo]
-:
-  (FB.ofBool p b).toBool varStore = b
-:= by
-  aesop (add simp [toBool,FB.ofBool,FB.true,FB.false])
-
-@[simp, grind =]
-lemma toBool_false
-  {varStore : VarStore p}
-:
-  (false p).toBool varStore = Bool.false
-:= by
-  simp [FB.false, FB.toBool]
-
-@[grind .]
-lemma toBool_eq_false_of_eval_eq
-  {varStore : VarStore p}
-  {x : FB p}
-  (h : [varStore|x =Γ false p])
-:
-  x.toBool varStore = .some Bool.false
-:= by
-  grind [FB.toBool, false]
-
-@[grind .]
-lemma toBool_of_eval_eq_eval_true
-  {varStore : VarStore p}
-  {x : FB p}
-  (h : [varStore|x =Γ true p])
-:
-  x.toBool varStore = .some Bool.true
-:= by
-  grind [FB.toBool, true]
-
-@[simp, grind =]
-lemma toBool_true
-  {varStore : VarStore p}
-:
-  (true p).toBool varStore = Bool.true
-:= by
-  simp [FB.true, FB.toBool]
-
-@[simp, grind .] -- TODO(provisional `simp`)
-lemma eval_ofBool_toBool_of_isValid
-  {p : ℕ}
-  {varStore : VarStore p}
-  {x: FB p}
-  (h : x.isValid varStore)
-  [p.AtLeastTwo]
-:
-  [varStore|(FB.ofBool p ((x.toBool varStore).get (by grind))) =Γ x]
-:= by
-  grind
-
-namespace ofBool
-
-lemma isAlwaysValid (b:Bool) : isAlwaysValid (FB.ofBool p b) := by
-  unfold FB.isAlwaysValid isValid FB.ofBool
-  aesop
-
-lemma equiv (varStore) (b) : FixedExp.eval varStore (ofBool p b) =
-  if b then .some 1 else .some 0
-:= by
-  simp [ofBool]
-  cases b
-  all_goals simp [FB.false, FB.true]
-
-end ofBool
-
-instance : IsValid p (FB p) := ⟨fun Γ a ↦ FB.isValid a Γ⟩
-
-omit [p.AtLeastTwo] in
-lemma isValid_iff {varStore} {x} :
-  IsValid.isValid (α := FB p) varStore x ↔
-  x.eval varStore = .some 0 ∨
-  x.eval varStore = .some 1 := by rfl
-
-instance {p} : VarStoreSize p (FB p) where
-  size := 1
-  toLinear varStore x := #v[x.eval varStore |>.getD 42]
-
-instance : Convert p (FB p) Bool where
-  toIdeal Γ x := FB.toBool x Γ
-  toRepresents := FB.ofBool p
-  isValid_iff_isSome_toIdeal Γ x := by unfold_projs; grind [IsValid.isValid]
-  toIdeal_toRepresents := by simp
-  toRepresents_toIdeal := by simp
-
-/-
-TODO Provisional simp
--/
-attribute [simp, grind =] Convert.toIdeal_toRepresents Convert.toRepresents_toIdeal
-
-lemma toIdeal_def {varStore} {x} :
-  Convert.toIdeal (representsT := FB p) (idealT := Bool) varStore x =
-  (FB.toBool x varStore) := rfl
-
-lemma toRepresents_def {x} :
-  Convert.toRepresents p (representsT := FB p) (idealT := Bool) x =
-  FB.ofBool p x := rfl
-
-@[grind .]
-lemma isValid_iff_exists_eq_eval
-  {x : FB p} {varStore : VarStore p}
-:
-  x.isValid varStore ↔ ∃ b, [varStore|x =Γ FB.ofBool p b]
-:= by
-  simp [isValid, eval_true, eval_false]
-
-omit [p.AtLeastTwo] in
-@[grind ←]
-lemma toBool_eq_none_of_eval_eq_none
-  {x : FB p} {varStore : VarStore p}
-  (h : [varStore|x] = .none)
-:
-  (x.toBool varStore = .none)
-:= by
-  grind [FB.toBool]
-
-@[grind .]
-lemma not_IsValid_of_toBool_eq_none
-  {x : FB p} {varStore : VarStore p}
-  (h : x.toBool varStore = .none)
-:
-  ¬IsValid.isValid varStore x
-:= by
-  unfold_projs
-  grind
-
-@[grind! .]
-lemma IsValid_iff_toBool_isSome
-  {x : FB p} {varStore : VarStore p}
-:
-  (x.toBool varStore).isSome ↔
-  IsValid.isValid varStore x
-:= by
-  unfold_projs
-  grind
-
--- -- This is breaking the instance abstraction layer
--- -- and secretly proving something only about the specific
--- -- Convert FB p Bool instance isn't it?
--- -- Seems bad
--- @[grind .]
--- lemma toIdeal_isSome_of_eval_eq_true
---   {varStore : VarStore p}
---   {a : FB p}
---   (h : [varStore|a =Γ true p])
--- :
---   (Convert.toIdeal (idealT := Bool) varStore a).isSome = Bool.true
+-- @[grind =]
+-- lemma eval_true {p : ℕ} {varStore : VarStore p} [p.AtLeastTwo]:
+--   [varStore|true p] = .some 1
 -- := by
---   have := Convert.isValid_iff_isSome_toIdeal varStore a (idealT := Bool)
---   rw [this.mp]
---   have := isValid_iff_exists_eq_eval (x := a) (varStore := varStore)
+--   simp [FB.true]
+
+-- @[grind =]
+-- lemma eval_false {p : ℕ} {varStore : VarStore p} [p.AtLeastTwo]:
+--   [varStore|false p] = .some 0
+-- := by
+--   simp [FB.false]
+
+-- @[simp, grind =]
+-- lemma eval_true_isSome {p : ℕ} {varStore : VarStore p} [p.AtLeastTwo]:
+--   [varStore|true p].isSome = Bool.true
+-- := by
+--   grind
+
+-- @[simp, grind =]
+-- lemma eval_false_isSome {p : ℕ} {varStore : VarStore p} [p.AtLeastTwo]:
+--   [varStore|false p].isSome = Bool.true
+-- := by
+--   grind
+
+-- variable {p : ℕ} [p.AtLeastTwo]
+
+-- def isValid (x : FB p) (varStore : VarStore p) : Prop :=
+--   x.eval varStore = .some 0 ∨
+--   x.eval varStore = .some 1
+
+-- -- TODO there must be a better way of putting this
+-- -- Well, this is just `isValid_iff` with an extra step.
+-- -- I think this is good, and it `simp`s down to `true | false` via `eval_<t|f>`.
+-- @[grind .]
+-- lemma isValid_iff_eval_eq_eval_false_or_eval_true
+--   {x : FB p} {varStore : VarStore p}
+-- :
+--   x.isValid varStore ↔ (
+--     [varStore|x =Γ false p] ∨
+--     [varStore|x =Γ true p]
+--   )
+-- := by
+--   simp [isValid, eval_true, eval_false]
+
+-- def isAlwaysValid (x : FB p) : Prop :=
+--   ∀ varStore, x.isValid varStore
+
+-- def toBool (x : FB p) (varStore : VarStore p) : Option Bool :=
+--   [varStore|x].bind (λ x => if x == 1 then Bool.true else if x == 0 then Bool.false else .none)
+
+-- @[grind .]
+-- lemma toBool_isSome_eq_true_of_isValid
+--   {x : FB p} {varStore : VarStore p}
+--   (h_isValid : x.isValid varStore)
+-- :
+--   (x.toBool varStore).isSome = Bool.true
+-- := by
+--   grind [toBool]
+
+-- omit [p.AtLeastTwo] in
+-- @[grind .]
+-- lemma toBool_isSome_eq_false_of_isValid
+--   {x : FB p} {varStore : VarStore p}
+--   (h_isValid : ¬x.isValid varStore)
+-- :
+--   (x.toBool varStore).isSome = Bool.false
+-- := by
+--   simp [isValid] at h_isValid
+--   unfold toBool
+--   set y := [varStore|x]
+--   obtain _ | ⟨y⟩ := y <;> grind
+
+-- def ofBool (p : ℕ) [p.AtLeastTwo] (x : Bool) : FB p :=
+--   if x then FB.true p else FB.false p
+
+-- @[simp, grind =]
+-- lemma eval_ofBool {p : ℕ} {varStore : VarStore p} [p.AtLeastTwo] {b : Bool} :
+--   [varStore|ofBool p b] = if b then [varStore|true p] else [varStore|false p]
+-- := by
+--   grind [FB.ofBool]
+
+-- @[simp, grind =]
+-- lemma toBool_ofBool
+--   {p : ℕ}
+--   {varStore : VarStore p}
+--   (b: Bool)
+--   [p.AtLeastTwo]
+-- :
+--   (FB.ofBool p b).toBool varStore = b
+-- := by
+--   aesop (add simp [toBool,FB.ofBool,FB.true,FB.false])
+
+-- @[simp, grind =]
+-- lemma toBool_false
+--   {varStore : VarStore p}
+-- :
+--   (false p).toBool varStore = Bool.false
+-- := by
+--   simp [FB.false, FB.toBool]
+
+-- @[grind .]
+-- lemma toBool_eq_false_of_eval_eq
+--   {varStore : VarStore p}
+--   {x : FB p}
+--   (h : [varStore|x =Γ false p])
+-- :
+--   x.toBool varStore = .some Bool.false
+-- := by
+--   grind [FB.toBool, false]
+
+-- @[grind .]
+-- lemma toBool_of_eval_eq_eval_true
+--   {varStore : VarStore p}
+--   {x : FB p}
+--   (h : [varStore|x =Γ true p])
+-- :
+--   x.toBool varStore = .some Bool.true
+-- := by
+--   grind [FB.toBool, true]
+
+-- @[simp, grind =]
+-- lemma toBool_true
+--   {varStore : VarStore p}
+-- :
+--   (true p).toBool varStore = Bool.true
+-- := by
+--   simp [FB.true, FB.toBool]
+
+-- @[simp, grind .] -- TODO(provisional `simp`)
+-- lemma eval_ofBool_toBool_of_isValid
+--   {p : ℕ}
+--   {varStore : VarStore p}
+--   {x: FB p}
+--   (h : x.isValid varStore)
+--   [p.AtLeastTwo]
+-- :
+--   [varStore|(FB.ofBool p ((x.toBool varStore).get (by grind))) =Γ x]
+-- := by
+--   grind
+
+-- namespace ofBool
+
+-- lemma isAlwaysValid (b:Bool) : isAlwaysValid (FB.ofBool p b) := by
+--   unfold FB.isAlwaysValid isValid FB.ofBool
+--   aesop
+
+-- lemma equiv (varStore) (b) : FixedExp.eval varStore (ofBool p b) =
+--   if b then .some 1 else .some 0
+-- := by
+--   simp [ofBool]
+--   cases b
+--   all_goals simp [FB.false, FB.true]
+
+-- end ofBool
+
+-- instance : IsValid p (FB p) := ⟨fun Γ a ↦ FB.isValid a Γ⟩
+
+-- omit [p.AtLeastTwo] in
+-- lemma isValid_iff {varStore} {x} :
+--   IsValid.isValid (α := FB p) varStore x ↔
+--   x.eval varStore = .some 0 ∨
+--   x.eval varStore = .some 1 := by rfl
+
+-- instance {p} : VarStoreSize p (FB p) where
+--   size := 1
+--   toLinear varStore x := #v[x.eval varStore |>.getD 42]
+
+-- instance : Convert p (FB p) Bool where
+--   toIdeal Γ x := FB.toBool x Γ
+--   toRepresents := FB.ofBool p
+--   isValid_iff_isSome_toIdeal Γ x := by unfold_projs; grind [IsValid.isValid]
+--   toIdeal_toRepresents := by simp
+--   toRepresents_toIdeal := by simp
+
+-- /-
+-- TODO Provisional simp
+-- -/
+-- attribute [simp, grind =] Convert.toIdeal_toRepresents Convert.toRepresents_toIdeal
+
+-- lemma toIdeal_def {varStore} {x} :
+--   Convert.toIdeal (representsT := FB p) (idealT := Bool) varStore x =
+--   (FB.toBool x varStore) := rfl
+
+-- lemma toRepresents_def {x} :
+--   Convert.toRepresents p (representsT := FB p) (idealT := Bool) x =
+--   FB.ofBool p x := rfl
+
+-- @[grind .]
+-- lemma isValid_iff_exists_eq_eval
+--   {x : FB p} {varStore : VarStore p}
+-- :
+--   x.isValid varStore ↔ ∃ b, [varStore|x =Γ FB.ofBool p b]
+-- := by
+--   simp [isValid, eval_true, eval_false]
+
+-- omit [p.AtLeastTwo] in
+-- @[grind ←]
+-- lemma toBool_eq_none_of_eval_eq_none
+--   {x : FB p} {varStore : VarStore p}
+--   (h : [varStore|x] = .none)
+-- :
+--   (x.toBool varStore = .none)
+-- := by
+--   grind [FB.toBool]
+
+-- @[grind .]
+-- lemma not_IsValid_of_toBool_eq_none
+--   {x : FB p} {varStore : VarStore p}
+--   (h : x.toBool varStore = .none)
+-- :
+--   ¬IsValid.isValid varStore x
+-- := by
 --   unfold_projs
 --   grind
 
--- @[grind .]
--- lemma toIdeal_isSome_of_eval_eq_false
---   {varStore : VarStore p}
---   {a : FB p}
---   (h : [varStore|a =Γ false p])
+-- @[grind! .]
+-- lemma IsValid_iff_toBool_isSome
+--   {x : FB p} {varStore : VarStore p}
 -- :
---   (Convert.toIdeal (idealT := Bool) varStore a).isSome = Bool.true
+--   (x.toBool varStore).isSome ↔
+--   IsValid.isValid varStore x
 -- := by
---   have := Convert.isValid_iff_isSome_toIdeal varStore a (idealT := Bool)
---   rw [this.mp]
---   have := isValid_iff_exists_eq_eval (x := a) (varStore := varStore)
 --   unfold_projs
 --   grind
 
--- @[grind =]
--- lemma toIdeal_true_iff_eval_eq_true
---   {varStore : VarStore p}
---   {a : FB p}
--- :
---   ([varStore|a =Γ true p]) ↔
---   ((Convert.toIdeal varStore a) = .some Bool.true)
--- := by
---   unfold_projs
---   simp [toBool]
---   obtain _ | x := [varStore|a]
---   <;> grind
+-- -- -- This is breaking the instance abstraction layer
+-- -- -- and secretly proving something only about the specific
+-- -- -- Convert FB p Bool instance isn't it?
+-- -- -- Seems bad
+-- -- @[grind .]
+-- -- lemma toIdeal_isSome_of_eval_eq_true
+-- --   {varStore : VarStore p}
+-- --   {a : FB p}
+-- --   (h : [varStore|a =Γ true p])
+-- -- :
+-- --   (Convert.toIdeal (idealT := Bool) varStore a).isSome = Bool.true
+-- -- := by
+-- --   have := Convert.isValid_iff_isSome_toIdeal varStore a (idealT := Bool)
+-- --   rw [this.mp]
+-- --   have := isValid_iff_exists_eq_eval (x := a) (varStore := varStore)
+-- --   unfold_projs
+-- --   grind
 
--- @[grind =]
--- lemma eval_eq_false_iff_toIdeal_eq_false
---   {varStore : VarStore p}
---   {a : FB p}
--- :
---   ([varStore|a] = [varStore|false p]) ↔
---   ((Convert.toIdeal varStore a) = .some Bool.false)
--- := by
---   unfold_projs
---   simp [toBool]
---   obtain _ | x := [varStore|a]
---   <;> grind
+-- -- @[grind .]
+-- -- lemma toIdeal_isSome_of_eval_eq_false
+-- --   {varStore : VarStore p}
+-- --   {a : FB p}
+-- --   (h : [varStore|a =Γ false p])
+-- -- :
+-- --   (Convert.toIdeal (idealT := Bool) varStore a).isSome = Bool.true
+-- -- := by
+-- --   have := Convert.isValid_iff_isSome_toIdeal varStore a (idealT := Bool)
+-- --   rw [this.mp]
+-- --   have := isValid_iff_exists_eq_eval (x := a) (varStore := varStore)
+-- --   unfold_projs
+-- --   grind
 
-/--
-Just like `@[simp] _root_.Option.bind_eq` says `Bind.bind a b = Option.bind a b`.
--/
-@[simp, grind =]
-lemma toIdeal_eq {p : ℕ} [p.AtLeastTwo] {varStore : VarStore p} {x : FB p} :
-  (Convert.toIdeal (representsT := FB p) (idealT := Bool)) varStore x =
-  x.toBool varStore := rfl
+-- -- @[grind =]
+-- -- lemma toIdeal_true_iff_eval_eq_true
+-- --   {varStore : VarStore p}
+-- --   {a : FB p}
+-- -- :
+-- --   ([varStore|a =Γ true p]) ↔
+-- --   ((Convert.toIdeal varStore a) = .some Bool.true)
+-- -- := by
+-- --   unfold_projs
+-- --   simp [toBool]
+-- --   obtain _ | x := [varStore|a]
+-- --   <;> grind
+
+-- -- @[grind =]
+-- -- lemma eval_eq_false_iff_toIdeal_eq_false
+-- --   {varStore : VarStore p}
+-- --   {a : FB p}
+-- -- :
+-- --   ([varStore|a] = [varStore|false p]) ↔
+-- --   ((Convert.toIdeal varStore a) = .some Bool.false)
+-- -- := by
+-- --   unfold_projs
+-- --   simp [toBool]
+-- --   obtain _ | x := [varStore|a]
+-- --   <;> grind
+
+-- /--
+-- Just like `@[simp] _root_.Option.bind_eq` says `Bind.bind a b = Option.bind a b`.
+-- -/
+-- @[simp, grind =]
+-- lemma toIdeal_eq {p : ℕ} [p.AtLeastTwo] {varStore : VarStore p} {x : FB p} :
+--   (Convert.toIdeal (representsT := FB p) (idealT := Bool)) varStore x =
+--   x.toBool varStore := rfl
 
 end FB
 
-end Clap.Edsl.Lang
+end Clap.Lang
