Clap/eDSLState/Convert.lean
@@ -1,0 +1,64 @@
+import Clap.eDSLState.IsValid
+
+namespace Clap
+
+class Convert (p : ℕ) (representsT idealT : Type) extends IsValid p representsT where
+  toIdeal : (VarStore p) → (HashConsSt p) → representsT → Option idealT
+  toRepresents : idealT → HashConsM p representsT
+  isValid_iff_isSome_toIdeal :
+    ∀ (varStore : VarStore p) (σ : HashConsSt p) (x : representsT),
+      isValid varStore σ x ↔ (toIdeal varStore σ x).isSome
+  toIdeal_toRepresents :
+    ∀ (varStore : VarStore p) (σ : HashConsSt p) (x : idealT),
+      toIdeal varStore ((toRepresents x).run σ).2 ((toRepresents x).run σ).1 = .some x
+
+@[simp, grind =]
+lemma Convert.toRepresents_toIdeal
+  {p : ℕ}
+  {representsT idealT : Type}
+  [inst: Convert p representsT idealT]
+  {varStore : VarStore p}
+  {σ : HashConsSt p}
+  {x : representsT}
+  (h : IsValid.isValid varStore σ x)
+:
+  toIdeal varStore σ (toRepresents p (representsT := representsT) ((toIdeal (idealT := idealT) varStore σ x).get ((isValid_iff_isSome_toIdeal varStore x).mp h))) =
+  inst.toIdeal varStore σ x
+:= by
+  simp [inst.toIdeal_toRepresents]
+
+instance {p : ℕ} : Convert p Unit Unit where
+  isValid := fun _ _ _ ↦ True
+  toIdeal _ x := .some x
+  toRepresents x := x
+  isValid_iff_isSome_toIdeal _ _ := by grind
+  toIdeal_toRepresents _ _ := by grind
+
+@[simp, grind .]
+lemma isValid_iff_isSome_toIdeal {p} {α β : Type} [Convert p α β]
+  {varStore : VarStore p} {σ : HashConsSt p} {x : α}
+:
+  (Convert.toIdeal (idealT := β) varStore x).isSome ↔
+  IsValid.isValid varStore σ x
+:= by
+  aesop (add safe cases Convert)
+
+@[grind .]
+lemma isValid_of_toIdeal_eq_some {p} {α β : Type} [Convert p α β]
+  {varStore : VarStore p} {x : α} {b : β}
+  (h : (Convert.toIdeal (idealT := β) varStore x) = .some b)
+:
+  IsValid.isValid varStore x
+:= by
+  have := Option.isSome_of_eq_some h
+  grind
+
+@[simp, grind .]
+lemma toIdealtoRepresents_of_convert {p} {α β : Type} [Convert p α β]
+  {varStore : VarStore p} {x : β}
+:
+  Convert.toIdeal (representsT := α) varStore (Convert.toRepresents p x) = .some x
+:= by
+  aesop (add safe cases Convert)
+
+end Clap
