Clap/eDSLState/IsValid.lean
@@ -1,0 +1,41 @@
+import Mathlib.Data.ZMod.Basic
+import Clap.eDSLState.Monad
+import Clap.eDSLState.Varstore
+
+namespace Clap
+
+class IsValid (p : ℕ) (α : Type) where
+  isValid : VarStore p → HashConsSt p → α → Prop
+
+class VarStoreSize (p : ℕ) (α : Type) where
+  size : ℕ
+  toLinear : (VarStore p) → α → Vector (ZMod p) size
+
+attribute [reducible] VarStoreSize.size
+
+instance instVarStoreSizeUnit {p : ℕ} : VarStoreSize p Unit where
+  size := 0
+  toLinear _ _ := #v[]
+
+@[grind =]
+lemma instVarStoreSizeUnit_size {p : ℕ}:
+  (@instVarStoreSizeUnit p).size = 0
+:= rfl
+
+@[grind =]
+lemma instVarStoreSizeUnit_size' {p : ℕ}:
+  @VarStoreSize.size p Unit instVarStoreSizeUnit = 0
+:= rfl
+
+-- set_option pp.all true in
+@[grind =]
+lemma instVarStoreSizeUnit_toLinear
+  {p : ℕ}
+  {varStore : VarStore p}
+  {x : Unit}
+:
+  (@instVarStoreSizeUnit p).toLinear varStore x =
+  @Vector.mk _ 0 #[] (by simp)
+:= rfl
+
+end Clap
